Moved compute_expr from Clight_lemmas.v to expr.v,   renamed it/change arguments to eval_expr rho...
Changed typecheker to return a tc_assert, 
  a list of assertions that must be satisfied 
  to show that an expression evaluation completes

Modified typechecking soundness to include denote_tc_assert
  on the result of the typecheker run, commented soundness
  proof for now. I have more typechecker work to do before
  I work on the proof again.

Changed typecheck_statement to a parameter for now, since
  I don't think we need to show that we guarantee a 
  successful step with typecheck_statement, I need to figure
  out the "non-strict" expr typechecker befor I implement
  this. I think a function that makes sure there is no
  tc_FF in a tc assert will work.

Defined func_tycontext

veric/expr.v
@@ -6,14 +6,65 @@ Require Import msl.rmaps_lemmas.
 Require Import veric.compcert_rmaps.
 Require Import veric.Clight_lemmas.
 
-Definition eval_expr (rho: environ) (e: expr) : val :=
-   compute_expr (ge_of rho) (ve_of rho) (te_of rho) e.
+Fixpoint eval_expr (rho:environ) (e: expr) : val :=
+ match e with
+ | Econst_int i ty => Vint i
+ | Econst_float f ty => Vfloat f
+ | Etempvar id ty => force_val (PTree.get id (te_of rho))
+ | Eaddrof a ty => eval_lvalue rho a
+ | Eunop op a ty =>  force_val (sem_unary_operation op (eval_expr rho a) (typeof a))
+ | Ebinop op a1 a2 ty =>  
+         force_val (sem_binary_operation op
+                    (eval_expr rho a1) (typeof a1)
+                    (eval_expr rho a2) (typeof a2)
+                    (fun _ _ => false))
+ | Econdition a1 a2 a3 ty => 
+    match bool_val (eval_expr rho a1) (typeof a1) with
+    | Some true => force_val (sem_cast (eval_expr rho a2) (typeof a2) ty)
+    | Some false => force_val (sem_cast (eval_expr rho a3) (typeof a3) ty)
+    | None => Vundef
+    end
+ | Ecast a ty => force_val (sem_cast (eval_expr rho a) (typeof a) ty)
+ | _ => Vundef
+ end 
 
-Definition eval_lvalue (rho: environ) (e: expr) : val :=
-   compute_lvalue (ge_of rho) (ve_of rho) (te_of rho) e.
+ with eval_lvalue (rho: environ) (e: expr) : val := 
+ match e with 
+ | Evar id ty => match PTree.get id (ve_of rho) with
+                         | Some (b,ty') => if type_eq ty ty'
+                                                    then if negb (type_is_volatile ty')
+                                                       then Vptr b Int.zero else Vundef
+                                                    else Vundef
+                         | None => 
+                            match (ge_of rho) id with
+                            | Some (v,ty') => if type_eq ty ty' then v else Vundef
+                            | None => Vundef
+                            end
+                        end
+ | Ederef a ty => match eval_expr rho a with
+                        | Vptr l ofs => Vptr l ofs
+                        | _ => Vundef
+	          end
+ | Efield a i ty => match eval_expr rho a, typeof a with
+                            | Vptr l ofs, Tstruct id fList att =>
+                                  match field_offset i fList with 
+                                  | Errors.OK delta => Vptr l (Int.add ofs (Int.repr delta))
+                                  | _ => Vundef
+                                  end
+                            | Vptr l ofs, Tunion id fList att => Vptr l ofs
+                            | _, _ => Vundef
+                            end
+ | _  => Vundef
+ end.
+
 
 (*Temps, vars, function return*)
-Definition tycontext: Type := prod (prod (PTree.t type) (PTree.t type)) type.
+Definition tycontext: Type := (PTree.t (type * bool) * (PTree.t type) * type)%type.
+
+Definition empty_tycontext : tycontext := (PTree.empty (type * bool), PTree.empty type, Tvoid).
+
+Definition Delta1 : tycontext := (PTree.set 1%positive (type_int32s, false) (PTree.empty (type * bool)),
+                                 PTree.empty type, Tvoid).
 
 Definition temp_types (Delta: tycontext) := fst (fst Delta).
 Definition var_types (Delta: tycontext) := snd (fst Delta).
@@ -27,6 +78,8 @@ match ty with
 | Tfloat _ _ => true
 | _ => false
 end.
+(*Make sure I am using the above correctly!!!*)
+
 (*
 Parameter combine_types : type -> type -> option type .
 
@@ -62,7 +115,9 @@ end.
 (*Might need to include quite a few more!*)
 Definition is_pointer_type ty :=
 match ty with
-| Tpointer _ _ => true
+| (Tpointer _ _ | Tarray _ _ _ 
+                   | Tfunction _ _ | Tstruct _ _ _ 
+                   | Tunion _ _ _) => true
 | _ => false
 end.
 
@@ -84,112 +139,115 @@ match op with
                     end
 end.
 
-Definition isBinOpResultType op a1 a2 ty : bool :=
+Inductive tc_assert :=
+| tc_FF: tc_assert
+| tc_TT : tc_assert
+| tc_andp: tc_assert -> tc_assert -> tc_assert
+| tc_nonzero: expr -> tc_assert
+| tc_isptr: expr -> tc_assert
+| tc_range32: expr -> tc_assert.
+
+Definition tc_bool (b : bool) :=
+if b then tc_TT else tc_FF.
+
+
+(*TODO most tc_FF should be an assert of some sort (not default)*)
+Definition isBinOpResultType op a1 a2 ty : tc_assert :=
 match op with
   | Oadd => match classify_add (typeof a1) (typeof a2) with 
-                    | add_default => false
-                    | add_case_ii _ => is_int_type ty 
-                    | add_case_pi _ _ | add_case_ip _ _ => 
-                        is_pointer_type ty
-                    | _ => is_float_type ty
+                    | add_default => tc_FF
+                    | add_case_ii _ => tc_bool (is_int_type ty) 
+                    | add_case_pi _ _ | add_case_ip _ _ => tc_FF 
+                        (*is_pointer_type ty*)
+                    | _ => tc_bool (is_float_type ty)
                     end
   | Osub => match classify_sub (typeof a1) (typeof a2) with 
-                    | sub_default => false
-                    | sub_case_ii _ => is_int_type ty 
-                    | sub_case_pi _ => is_pointer_type ty
-                    | sub_case_pp _ => false
-                    | _ => is_float_type ty
+                    | sub_default => tc_FF
+                    | sub_case_ii _ => tc_bool (is_int_type ty) 
+                    | sub_case_pi _ => tc_FF (*is_pointer_type ty ... comment for now, until I figure out null issue*)
+                    | sub_case_pp _ => tc_FF
+                    | _ => tc_bool (is_float_type ty)
                     end 
   | Omul => match classify_mul (typeof a1) (typeof a2) with 
-                    | mul_default => false
-                    | mul_case_ii _ => is_int_type ty
-                    | _ => is_float_type ty
+                    | mul_default => tc_FF
+                    | mul_case_ii _ => tc_bool (is_int_type ty)
+                    | _ => tc_bool (is_float_type ty)
                     end 
-  | Omod | Odiv | Oshl | Oshr => false (*pushing this to command because of possible non-evaluation*)
+  | Omod | Odiv | Oshl | Oshr => tc_FF (*these need asserts, not done yet*)
   | Oand | Oor  | Oxor => match classify_binint (typeof a1) (typeof a2) with
-                          | binint_case_ii _ => is_int_type ty
-                          | _ => false
+                          | binint_case_ii _ =>tc_bool (is_int_type ty)
+                          | _ => tc_FF
                           end   
   | Oeq | One | Olt 
     | Ogt | Ole | Oge => 
        match classify_cmp (typeof a1) (typeof a2) with
-       | cmp_case_pp | cmp_default => false
-       | _ => is_int_type ty
+       | cmp_case_pp | cmp_default => tc_FF
+       | _ => tc_bool (is_int_type ty)
        end
 end.
 
 
-Definition isCastResultType tfrom tto ty : bool :=
+Definition isCastResultType tfrom tto ty : tc_assert :=
 match classify_cast tfrom tto with
 | cast_case_default | 
-   cast_case_f2i _ _ => false
-| cast_case_neutral  => type_eq tfrom ty
+   cast_case_f2i _ _ => tc_FF (*figure out what this case is and assert it*)
+| cast_case_neutral  => if type_eq tfrom ty then tc_TT else tc_FF
 | _ => match tto with 
-      | Tint _ _ _  => is_int_type ty
-      | Tfloat _ _  => is_float_type ty
-      | _ => false
+      | Tint _ _ _  => tc_bool (is_int_type ty)
+      | Tfloat _ _  => tc_bool (is_float_type ty)
+      | _ => tc_FF
       end
 end.
 
-
 (* NOTE: typecheck_expr allows only _pure_ expressions that don't access the heap if pure=true *)
-Fixpoint typecheck_expr_pure (Delta : tycontext) (e: expr) : bool :=
-let tcr := typecheck_expr_pure Delta in
+Fixpoint typecheck_expr (Delta : tycontext) (e: expr) : tc_assert :=
+let tcr := typecheck_expr Delta in
 match e with
- | Econst_int _ (Tint _ _ _) => true 
- | Econst_float _ (Tfloat _ _) => true
+ | Econst_int _ (Tint _ _ _) => tc_TT 
+ | Econst_float _ (Tfloat _ _) => tc_TT
  | Etempvar id ty => match (temp_types Delta)!id with 
-                       | Some ty' => type_eq ty ty' 
-		       | None => false 
+                       | Some ty' => if type_eq ty (fst ty') then tc_TT else tc_FF 
+		       | None => tc_FF
                      end
- | Eaddrof a ty => typecheck_lvalue_pure Delta a && is_pointer_type (ty)
- | Eunop op a ty => (isUnOpResultType op a ty) && (tcr a)
- | Ebinop op a1 a2 ty => (isBinOpResultType op a1 a2 ty) && (tcr a1) && (tcr a2)
- | Econdition a1 a2 a3 ty => (tcr a1) && (tcr a2) && (tcr a3) && (is_skalar_type (typeof a1)) && (*int or pointer*)
-                              (isCastResultType (typeof a2) ty ty) && (isCastResultType (typeof a3) ty ty)
- | Ecast a ty => (tcr a) && isCastResultType (typeof a) (ty) ty
- | _ => false
+ | Eaddrof a ty => tc_andp (typecheck_lvalue Delta a) (tc_bool (is_pointer_type ty))
+ | Eunop op a ty => tc_andp (tc_bool (isUnOpResultType op a ty)) (tcr a)
+ | Ebinop op a1 a2 ty => tc_andp (tc_andp (isBinOpResultType op a1 a2 ty)  (tcr a1)) (tcr a2)
+ | Econdition a1 a2 a3 ty => tc_andp (tc_andp (tc_andp (tc_andp (tc_andp (tcr a1) (tcr a2)) (tcr a3)) 
+                              (tc_bool (is_skalar_type (typeof a1)))) (*int or float...*)
+                              (isCastResultType (typeof a2) ty ty)) (isCastResultType (typeof a3) ty ty)
+ | Ecast a ty => tc_andp (tcr a) (isCastResultType (typeof a) ty ty)
+ | _ => tc_FF
 end
 
-with typecheck_lvalue_pure (Delta: tycontext) (e: expr) : bool :=
+with typecheck_lvalue (Delta: tycontext) (e: expr) : tc_assert :=
 match e with
  | Evar id ty => match (var_types Delta) ! id with 
-                  | Some ty' => type_eq ty ty' && 
-                                negb (type_is_volatile ty')
-                  | None => false
+                  | Some ty' => tc_andp (if type_eq ty ty' then tc_TT else tc_FF) 
+                                (tc_bool (negb (type_is_volatile ty)))
+                  | None => tc_FF
                  end
- | Ederef a ty => typecheck_expr_pure Delta a && is_pointer_type (typeof a)
- | Efield a i ty => typecheck_expr_pure Delta a && match typeof a with
+ (*| Ederef a ty => typecheck_expr_pure Delta a && is_pointer_type (typeof a) --need proof it isn't null*) 
+ | Efield a i ty => tc_andp (typecheck_expr Delta a) (match typeof a with
                             | Tstruct id fList att =>
                                   match field_offset i fList with 
-                                  | Errors.OK delta => true
-                                  | _ => false
+                                  | Errors.OK delta => tc_TT
+                                  | _ => tc_FF
                                   end
-                            | Tunion id fList att => true
-                            | _ => false
-                            end
- | _  => false
+                            | Tunion id fList att => tc_TT
+                            | _ => tc_FF
+                            end)
+ | _  => tc_FF
 end.
 
-(*Declaring these for now so uses everywhere else match up...
-typecheck_expr with no boolean is the "pure" typecheck*)
-Definition typecheck_expr Delta e : bool :=
-typecheck_expr_pure Delta e.
+(*Definition typecheck_exprlist Delta := forallb (typecheck_expr Delta).*)
 
-Definition typecheck_lvalue Delta e : bool :=
-typecheck_lvalue_pure Delta e.
-
-Definition typecheck_exprlist Delta := forallb (typecheck_expr Delta).
-
-(*BE SURE TO CHECK IF INT SHOULD TYPE CHECK AS POINTER*)
 Definition typecheck_val (v: val) (ty: type) : bool :=
  match v, ty with
  | Vint i, Tint _ _ _ => true  (* Maybe this needs to be adjusted to account for
                                                the size of the int?  Maybe not? *)
- | Vfloat v, Tfloat _ _ => true (*  Maybe this needs to be adjusted, ditto *)
-(*I don't think this matters now, I believe an int should always be an int*)
- (*| Vint i, (Tpointer _ _ | Tarray _ _ _ | Tfunction _ _) => 
-                    negb (Int.eq i Int.zero) (*commented for now, double check *)*)
+ | Vfloat v, Tfloat _ _ => true (*  Maybe this needs to be adjusted, ditto *) 
+ | Vint i, (Tpointer _ _ | Tarray _ _ _ | Tfunction _ _) => 
+                    negb (Int.eq i Int.zero) 
  | Vptr b z,  (Tpointer _ _ | Tarray _ _ _ 
                    | Tfunction _ _ | Tstruct _ _ _ 
                    | Tunion _ _ _) => true
@@ -219,42 +277,51 @@ match vty with
  | (id,ty)::tl => match ve!id with
                   | Some (_,ty') => if type_eq ty ty' then 
                            typecheck_var_environ tl ve ge
-                           else match ge id with
-                                | Some (_, ty') => if type_eq ty ty' then 
+                           else false
+                  | None => match ge id with
+                                | Some (v, ty') => if type_eq ty ty' &&  
+                                                      typecheck_val v ty' &&
+                                                      is_pointer_type ty' then 
                                                    typecheck_var_environ tl ve ge else
                                                    false
                                 | None => false
                                 end
-                  | None => false
                   end
  | nil => true
 end.
 
+Definition remove_assignedness {A B C} (x: (A * (B*C))) := let (a,d) := x in
+let (b,c) := d in 
+(a,b).
+
 Definition typecheck_environ (env : environ) (Delta: tycontext) : bool :=
-typecheck_temp_environ (PTree.elements (temp_types Delta)) (te_of env) &&
+typecheck_temp_environ (map remove_assignedness (PTree.elements (temp_types Delta))) (te_of env) &&
 typecheck_var_environ (PTree.elements (var_types Delta)) (ve_of env) (ge_of env).
 
 Definition temp_element_correct (te : temp_env) :=
 (fun (tyconEl : (PTree.elt * type)) => let (id,elt) := tyconEl in
   match te ! id with
-  | Some v => True
+  | Some v => typecheck_val v elt = true
   | _ => False
 end). 
 
 Definition te_correct (te : temp_env) (Delta: tycontext) := Forall
   (temp_element_correct te)
-  (PTree.elements (temp_types Delta)).
+  (map remove_assignedness (PTree.elements (temp_types Delta))).
 
 Definition var_element_correct (ve: env) (ge:genviron) : 
 (PTree.elt * type) -> Prop :=
 (fun (varel : (PTree.elt * type)) => let (id,ty) := varel in
   match ve ! id with
-  | Some (_,ty') => if type_eq ty ty' then True else
-        match (ge id) with
-        | Some (_,ty2') => if type_eq ty ty2' then True else False 
+  | Some (_,ty') => if type_eq ty ty' then True else False
+  | None => match (ge id) with
+        | Some (v,ty2') => if type_eq ty ty2' && 
+                              typecheck_val v ty2' &&
+                              is_pointer_type ty2'(*Double check===================================*)
+                              (*^will be correct with change to base.v*)
+        then True else False 
         | None => False
         end
-  | None => False
   end).
 
 Definition ve_correct (ve:env) (ge:genviron) (Delta: tycontext) :=
@@ -262,28 +329,101 @@ Forall (var_element_correct ve ge) (PTree.elements (var_types Delta)).
 
 
 Lemma typecheck_environ_sound : forall ge te ve Delta,
-(*Incomplete, final lemma will have ge_correct and ve correct
-maybe not... at least in pure mode*)
 typecheck_environ (mkEnviron ge ve te) Delta = true ->
-te_correct te Delta.
+te_correct te Delta /\ ve_correct ve ge Delta.
 Proof.
 intros.
 unfold typecheck_environ in *. destruct Delta. destruct p.
-unfold te_correct.
-unfold temp_types in *. simpl in *. induction (PTree.elements t0).
-auto.
+unfold te_correct. unfold ve_correct.
+unfold temp_types in *. simpl in *. split.
+
+induction (PTree.elements t0).
+constructor. 
 unfold temp_element_correct.
-simpl in *. destruct a. rewrite Forall_forall; intros.
-destruct x. simpl in H0. destruct H0. inv H0. destruct (te!e). auto. inv H.
-destruct (te!p). remember (typecheck_val v t2). destruct b0. 
+simpl in *. destruct a. destruct p0. rewrite Forall_forall; intros.
+destruct x. simpl in *. destruct H0. inv H0. destruct (te!e). 
+destruct (typecheck_val v t3). auto. inv H. inv H.
+destruct (te!p). remember (typecheck_val v t2). destruct b1. 
 intuition. rewrite Forall_forall in *. unfold temp_element_correct in *.
 specialize (H1 (e,t3)). intuition. inv H. inv H.
+
+unfold var_types in *; simpl in *. rewrite andb_true_iff in H. destruct H.
+clear H. rewrite Forall_forall. intros. 
+destruct x. induction (PTree.elements t1). inv H.
+simpl in *. destruct a. destruct H. inv H. destruct (ve !e). destruct p.
+destruct (type_eq t2 t3). auto. inv H0. destruct (ge e). destruct p.
+destruct (type_eq t2 t3 && typecheck_val v t3 && is_pointer_type t3). auto.
+intuition. inv H0. 
+apply IHl.
+clear IHl.  destruct (ve ! p). destruct p0. 
+destruct (type_eq t3 t4). subst.
+auto. inv H0. destruct (ge p). destruct p0. 
+destruct (type_eq t3 t4 && typecheck_val v t4 && is_pointer_type t4).
+auto. inv H0. inv H0. auto. 
+Qed.
+
+Lemma typecheck_te_sound : forall dv te,
+typecheck_temp_environ dv te = true ->
+Forall (temp_element_correct te) dv.
+Proof.
+intros. induction dv. auto.
+simpl in *. destruct a. remember (te! p). destruct o; auto.
+remember (typecheck_val v t). destruct b0. 
+rewrite Forall_forall. intros. simpl in H0. destruct H0. inv H0.
+unfold temp_element_correct. rewrite <- Heqo. auto. intuition.
+rewrite Forall_forall in H1. apply H1. auto. inv H. inv H.
 Qed.
 
 Lemma in_fst_in : forall A B (L : list (A*B)) (a:A) (b:B), In (a, b) L  -> In a (map (@fst A B) L) .
 Proof.
 intros A B L. induction L; intros. auto. simpl in *. inv H. auto. right. eapply IHL. apply H0.
 Qed.
+
+Lemma in_rem_in : forall A B C (L : list (A*(B*C))) a b c,
+In (a, (b, c)) L -> In (a,b) (map remove_assignedness (L)).
+intros A B C L. induction L; intros. inv H. simpl in *.
+inv H. left. auto. right. eapply  IHL. eauto.
+Qed.
+
+(*I think I need this eventually
+but can't figure it out right now...
+Lemma typecheck_environ_put_te : forall ge te ve Delta id v ,
+typecheck_environ (mkEnviron ge ve te) Delta = true ->
+(*((temp_types Delta) ! id = Some t ->
+  (typecheck_val v (fst t)) = true) ->*)
+(*typecheck_expr Delta (Etempvar id (typeof e)) = true ->
+typecheck_expr Delta e = true ->*) 
+typecheck_environ (mkEnviron ge ve (PTree.set id v te)) Delta = true.
+Proof.
+intros. unfold typecheck_environ in *. simpl in *. repeat rewrite andb_true_iff in *.
+intuition. clear H1. destruct Delta. destruct p. unfold temp_types in *; simpl in *.
+
+remember (map remove_assignedness (PTree.elements t0)).
+generalize dependent t0.
+induction l; intros; auto.
+
+simpl in *. destruct  a.  
+remember (te ! p). destruct o; intuition.
+remember (typecheck_val v0 t2). destruct b0; intuition.
+remember ((PTree.set id v te) ! p).
+destruct o. remember (typecheck_val v1 t2). destruct b0.
+eapply H.
+Focus 2. clear H.
+assert (typecheck_val v1 t2 = true). 
+apply typecheck_te_sound in H0. rewrite Forall_forall in *.
+unfold temp_element_correct in H0.
+clear Heqb1. 
+
+Focus 3. clear H.   
+assert (In (p,t3) (p,t3::l)).
+assert (x:=eq_dec p id). destruct x. subst. rewrite PTree.gss in Heqo0.
+inv Heqo0. apply typecheck_te_sound in H1. rewrite Forall_forall in H1.
+unfold temp_element_correct in H1.
+
+unfold typecheck_temp_environ in H. 
+ rewrite typecheck_environ_sound in H1. 
+*)
+
 
 
 Lemma no_rep_in_pair : forall A B L a b b2, list_norepet (map (@fst A B) (L)) ->
@@ -325,7 +465,17 @@ intros.
 destruct t; auto.
 Qed.
 
+Fixpoint denote_tc_assert (a: tc_assert) (rho: environ): Prop :=
+  match a with
+  | tc_FF => False
+  | tc_TT => True
+  | tc_andp b c => denote_tc_assert b rho /\ denote_tc_assert c rho
+  | tc_nonzero e => match eval_expr rho e with Vint i => if negb (Int.eq i Int.zero) then True else False
+                                               | _ => False end
+  | _ => False
+  end.
 
+(*come back here
 Lemma typecheck_binop_sound:
 forall (Delta : tycontext) (rho : environ) (b0 : binary_operation)
   (e1 e2 : expr) (t : type),
@@ -349,61 +499,87 @@ do 2
 (match goal with
 | [ |- context[(typeof ?X)]] => let x := fresh "tofx" in remember (typeof X) as x; destruct x
 end); intuition; simpl;
-try destruct i; try destruct s; try destruct i0; try destruct s0; intuition;(
+try solve [try destruct i; try destruct s; try destruct i0; try destruct s0; intuition;(
 simpl in *;
 try solve [do 2 try
 match goal with
 | [ |- context[compute_expr ?ge ?ve ?te ?e]] => remember (compute_expr ge ve te e) as compR; destruct compR
-end; try destruct t; auto; intuition; try (of_bool_destruct; auto)])). 
-Qed.*)
+end; try destruct t; auto; intuition; try (of_bool_destruct; auto)])]). 
+Qed.*) *)
 
 Lemma typecheck_both_sound: 
-  forall Delta rho e, 
+  forall Delta rho e P, 
              typecheck_environ rho Delta = true -> 
-             (typecheck_expr Delta e = true ->
+             (typecheck_expr Delta e = P ->
+              denote_tc_assert P rho ->
              typecheck_val (eval_expr rho e) (typeof e) = true) /\
-             (typecheck_lvalue Delta e = true -> 
-             typecheck_val (eval_lvalue rho e) (Tpointer Tvoid noattr)=true).
+             (forall pt, typecheck_lvalue Delta e = P -> 
+             denote_tc_assert P rho ->
+             is_pointer_type pt = true -> 
+             typecheck_val (eval_lvalue rho e) pt=true).
 Proof.
 intros. induction e; intuition.
+Admitted. (*So I can get it committed
+(*Const int*)
 simpl. destruct t; auto; simpl in H0; inv H0; intuition.
 
+(*Const float*)
 simpl in *. destruct t; intuition. 
 
+(*Var*)
 simpl in *. unfold eval_lvalue. simpl.
 
- admit. (*________________Finish when typecheck-environ is done*)
+apply typecheck_environ_sound in H. destruct H.
+clear H. unfold ve_correct in H2. rewrite Forall_forall in *.
+unfold var_element_correct in *.
+remember ((var_types Delta) ! i). destruct o; intuition. rewrite andb_true_iff in *.
+intuition. apply type_eq_true in H. subst. symmetry in Heqo.
+apply PTree.elements_correct in Heqo.
+specialize (H2 (i,t0)). intuition.
+remember ((ve_of rho) ! i). destruct o.
+destruct p. remember (type_eq t0 t). destruct s; intuition.
+subst. rewrite H3. destruct pt; auto.
+destruct (ge_of rho i); auto. destruct p. 
+remember (@proj_sumbool (t0 = t) (t0 = t -> False) (type_eq t0 t) &&
+       typecheck_val v t && is_pointer_type t).
+destruct b0; try contradiction. symmetry in Heqb0. repeat rewrite andb_true_iff in *. intuition.
+destruct (type_eq t0 t); auto. subst. admit.
+(*Stuck. If an int can typecheck as a pointer, should it be able to
+check as struct and union in the same cases??*)
+ (* Focus 2. destruct v; 
+destruct t; auto; intuition. destruct pt; intuition. 
 
-(*tempvar*)
-admit. (*________________________________________________________Also need to figure out typecheck-environ*)
-(* simpl in *. destruct rho. apply typecheck_environ_sound in H. 
-unfold te_correct in *. unfold te_complete in *. unfold type_element_correct in *.
-unfold type_element_complete in *. intuition. rewrite Forall_forall in *. 
+
+simpl in *. simpl in H5. simpl in *. simpl in *.
+ destruct t; auto.
+destruct t; auto.
+auto.*)
+
+(*Temp*)
+simpl in *. destruct rho. apply typecheck_environ_sound in H. intuition. 
+unfold te_correct in *. unfold temp_element_correct in *.
+rewrite Forall_forall in *. clear H2. 
 
 unfold eval_expr. unfold compute_expr. simpl. unfold force_val.
-remember (te ! i). destruct o. remember (Delta ! i). destruct o.
-  symmetry in Heqo0. apply PTree.elements_correct in Heqo0. specialize (H1 (i,v)).
-  symmetry in Heqo. apply PTree.elements_correct in Heqo. intuition.
-  specialize (H2 (i,t0)). intuition. remember (te ! i).  destruct o; auto.
-  remember (Delta ! i); destruct o; auto. remember (type_eq t t0).
-  destruct s; intuition. subst. clear H0. clear Heqs. symmetry in Heqo2. 
-  apply PTree.elements_correct in Heqo2. 
-  assert (norep := PTree.elements_keys_norepet Delta). 
-    assert (t0 = t1). eapply no_rep_in_pair; eauto. subst; auto.
-  intuition. remember (Delta ! i). destruct o. symmetry in Heqo0. 
-  apply PTree.elements_correct in Heqo0. specialize (H2 (i,t0)). intuition.
-  rewrite <- Heqo in H. intuition. intuition.
-*)
+destruct Delta. destruct p. 
+unfold temp_types in *. simpl in *.
+remember (t1 ! i). destruct o.
+  symmetry in Heqo. apply PTree.elements_correct in Heqo. 
+  destruct p. specialize (H1 (i,t3)). simpl in H1.
+apply type_eq_true in H0. inv H0. simpl in *.
+apply in_rem_in in Heqo. intuition. destruct (te ! i); auto.
+inv H0.  
 
-(*deref*)
+(*deref  -- no proof now, doesn't typecheck
 simpl in *. rewrite andb_true_iff in *; intuition. 
 unfold eval_lvalue. simpl. unfold eval_expr in *.
 remember (compute_expr (ge_of rho) (ve_of rho) (te_of rho) e).
-destruct v; intuition; destruct (typeof e); intuition. 
+destruct v; intuition; destruct (typeof e); intuition. simpl in *. 
+*)
 
 (*addrof*)
 unfold eval_expr in *. simpl in *. rewrite andb_true_iff in *; intuition. 
-destruct t; intuition.
+destruct t. Focus 4. simpl in *. apply H2. unfold typecheck_lvalue_pure in *.a
 
 (*Unop*)
 simpl in *. rewrite andb_true_iff in *. intuition.
@@ -469,16 +645,15 @@ remember (typeof e); destruct t0; intuition.
 
 remember (field_offset i f). destruct r; intuition.
 
-Qed. (*Threeish admits for figuring out type context!!-------------------------------*)
+Qed. *)
 
-
-
-Lemma typecheck_expr_sound : forall Delta rho e,
+Lemma typecheck_expr_sound : forall Delta rho e P,
  typecheck_environ rho Delta = true -> 
-             (typecheck_expr Delta e = true ->
+             (typecheck_expr Delta e = P ->
+              denote_tc_assert P rho ->
              typecheck_val (eval_expr rho e) (typeof e) = true).
-Proof.
-apply typecheck_both_sound. Qed.
+Proof. intros. 
+assert (TC := typecheck_both_sound Delta rho e P). intuition. Qed.
 
 
 (*Figure out where this is used, would not hold when pointers typecheck as
@@ -499,6 +674,7 @@ Definition is_ptr_type (ty: type) : bool :=
   | _ => false
 end.
 
+(*Not going to work because of null pointer
 Lemma get_typed_ptr:
    forall v ty, 
                    typecheck_val v ty = true -> 
@@ -506,44 +682,108 @@ Lemma get_typed_ptr:
                       exists b, exists ofs, v = Vptr b ofs.
 Proof.
 intros; destruct v; destruct ty; inv H; eauto; inv H0.
-Qed.
+Qed.*)
 
-(*do we get (most of) this with a proof relating compute_expr to eval_expr?
-and existing soundness proofs?*)
+
 Lemma eval_expr_relate:
-  forall Delta ge rho e m,
+  forall Delta ge rho e m P,
               filter_genv ge = ge_of rho ->
               typecheck_environ rho Delta = true ->
-              typecheck_expr Delta e = true ->
+              typecheck_expr Delta e = P ->
+              denote_tc_assert P rho ->
               Clight_sem.eval_expr ge (ve_of rho) (te_of rho) m e  (eval_expr rho e).
 Admitted.
 
 Lemma eval_lvalue_relate:
-  forall Delta ge rho e m,
+  forall Delta ge rho e m P,
               filter_genv ge = ge_of rho ->
               typecheck_environ rho Delta = true ->
-              typecheck_lvalue Delta e = true ->
+              typecheck_lvalue Delta e = P ->
+              denote_tc_assert P rho ->
               exists b, exists ofs, 
               Clight_sem.eval_lvalue ge (ve_of rho) (te_of rho) m e b ofs /\
               eval_lvalue rho e = Vptr b ofs.
 Admitted. 
 
-Fixpoint typecheck_stmt (Delta: tycontext) (c: Clight.statement) {struct c} : bool :=
+Definition set_temp_assigned (Delta:tycontext) id :=
+match (temp_types Delta) ! id with
+| Some (ty, _) => ( PTree.set id (ty,true) (temp_types Delta)  
+                    , var_types Delta, ret_type Delta)
+| None => Delta (*Shouldn't happen *)
+end.
+
+Parameter join_tycon: tycontext -> tycontext -> tycontext.
+
+(*Definition bool_expr Delta e := typecheck_expr Delta e && is_skalar_type (typeof e).*)
+
+(*Rework when I figure out how non-pure typecheck will work now... probably just make sure there is
+no tc_FF in the assertion*)
+Parameter update_tycon : tycontext -> Clight.statement -> option tycontext.
+(*Fixpoint update_tycon (Delta: tycontext) (c: Clight.statement) {struct c} : option tycontext :=
  match c with
- | Clight.Sskip => true
- | Clight.Sassign e1 e2 => 
+ | Sskip | Scontinue | Sbreak => Some Delta
+ | Sassign e1 e2 => if
                           typecheck_expr Delta e1 &&
                           typecheck_expr Delta e2 &&
-                          true (* also check t1 matches t2 *)
- | Clight.Sset id e2 => 
-                          true &&
+                          isCastResultType (typeof e2) (typeof e1) (typeof e1)
+                    then Some Delta else None
+ | Sset id e2 => if
                           (typecheck_expr Delta e2  (* this case for pure expressions  *)
                           || typecheck_lvalue Delta e2)  (* this case for top-level loads *)
-                       &&   true (* also check t1 matches t2 *)
- | _ => true  (* et cetera *)
- end.
- 
-(* Admitted: move to expr.v *)
-Parameter func_tycontext: Clight.function -> tycontext.
+                          &&   true (* also check t1 matches t2, will need two cases like above*)
+                 then Some (set_temp_assigned Delta id) else None
+ | Ssequence s1 s2 =>match update_tycon Delta s1 with
+                    | Some Delta' => match update_tycon Delta' s2 with
+                                     | Some Delta'' => Some Delta''
+                                     | None => None
+                                     end
+                    | None => None
+                    end
+ | Sifthenelse b s1 s2 =>if bool_expr Delta b then
+                            match update_tycon Delta s1 with
+                            | Some Delta1 => match update_tycon Delta s2 with
+                                             | Some Delta2 => Some (join_tycon Delta1 Delta2)
+                                             | None => None
+                                             end
+                            | None => None      
+                            end
+                            else None
+ | Swhile b s1  => if bool_expr Delta b then option_map (fun _ => Delta) (update_tycon Delta s1) else None
+ | Sdowhile b s1 => if bool_expr Delta b then (update_tycon Delta s1) else None 
+ | Sfor' b inc body => if bool_expr Delta b then 
+                         match update_tycon Delta inc with
+                         | Some Delta' => match update_tycon Delta' body with
+                                          | Some Delta'' => Some Delta 
+                                          | None => None
+                                          end
+                         | None => None
+                         end 
+                       else None
+ | Sswitch e ls => if typecheck_labeled_statements Delta ls && typecheck_expr Delta e 
+                   then Some Delta else None
+ | _ => Some Delta  (* et cetera *)
+end*)
+
+(*with typecheck_labeled_statements Delta ls :=
+match ls with
+| LSdefault s => match update_tycon Delta s with Some _ => true | _ => false end
+| LScase int s ls => match update_tycon Delta s with 
+                     | Some _ => typecheck_labeled_statements Delta ls
+                     | None => false
+                     end
+end.*)                               
 
 
+
+Definition typecheck_stmt (Delta: tycontext) (c: statement) : bool :=
+match update_tycon Delta c with
+| Some _ => true
+| None => false
+end.
+
+Definition func_tycontext (func: function) : tycontext :=
+(fold_right (fun (temp : ident *type) tenv, let (id,ty):= temp in PTree.set id (ty,false) tenv) 
+  (PTree.empty (type * bool)) func.(fn_temps),
+fold_right (fun (var : ident * type) venv, let (id, ty) := var in PTree.set id ty venv) 
+   (PTree.empty type) func.(fn_vars) ,
+fn_return func).
